yalla/mell_Prop.v
@@ -1,4 +1,4 @@
-(** * Example of a concrete use of the yalla library: unit-free MELL *)
+(** * Example of a concrete use of the yalla library: unit-free MELL in Prop *)
 
 From Coq Require Import Morphisms.
 From OLlibs Require Import funtheory dectype List_more Permutation_more Permutation_Type_more.
@@ -49,7 +49,7 @@ end.
 
 Lemma mell2ll_inj : injective mell2ll.
 Proof.
-intros A. induction A; intros B Heq; destruct B; inversion Heq;
+intro A. induction A; intros [] [=];
   try apply IHA in H0; try apply IHA1 in H0; try apply IHA2 in H1; subst; reflexivity.
 Qed.
 
@@ -62,7 +62,7 @@ Proof. induction l as [ | a l IHl]; [ | cbn; rewrite IHl ]; reflexivity. Qed.
 Lemma mell2ll_map_wn_inv l1 l2 : map formulas.wn l1 = map mell2ll l2 ->
   exists l2', l2 = map wn l2' /\ l1 = map mell2ll l2'.
 Proof.
-induction l1 as [|a l1 IHl1] in l2 |- *; intros Heq; destruct l2; inversion Heq.
+induction l1 as [|a l1 IHl1] in l2 |- *; intro Heq; destruct l2; inversion Heq.
 - exists nil. split; reflexivity.
 - apply IHl1 in H1.
   destruct f; inversion H0. subst.
@@ -115,23 +115,22 @@ Definition pfrag_mell := @ll_def.mk_pfrag atom  ll_def.pcut_none ll_def.NoAxioms
 
 Lemma mell2mellfrag l : mell l -> inhabited (ll_def.ll pfrag_mell (map mell2ll l)).
 Proof.
-intros pi. induction pi; try ((try inversion IHpi); do 2 constructor; assumption); rewrite ? map_app.
-- apply Permutation_Permutation_transp in H.
-  induction H.
-  + inversion IHpi. constructor. assumption.
-  + inversion IHpi. constructor.
+intro pi. induction pi; try ((try inversion IHpi); do 2 constructor; assumption); rewrite ? map_app.
+- apply Permutation_Permutation_transp in H. induction H; destruct IHpi as [IHpi].
+  + constructor. assumption.
+  + constructor.
     eapply ll_def.ex_r; [ eassumption | ].
     apply Permutation_Type_map, Permutation_Type_app_head, Permutation_Type_swap.
   + apply IHPermutation_transp2.
     * apply Permutation_Permutation_transp in H.
       eapply ex_r; eassumption.
-    * apply IHPermutation_transp1; assumption.
-- inversion IHpi1. inversion IHpi2. constructor.
+    * apply IHPermutation_transp1; [ | constructor ]; assumption.
+- destruct IHpi1 as [IHpi1], IHpi2 as [IHpi2]. constructor.
   eapply ll_def.ex_r.
-  + apply (ll_def.tens_r X X0).
+  + exact (ll_def.tens_r IHpi1 IHpi2).
   + cbn. rewrite map_app.
     apply Permutation_Type_cons, Permutation_Type_app_comm. reflexivity.
-- inversion IHpi. constructor.
+- destruct IHpi. constructor.
   cbn. rewrite mell2ll_map_wn. apply ll_def.oc_r. rewrite <- mell2ll_map_wn. assumption.
 Qed.
 
@@ -139,10 +138,11 @@ Lemma mellfrag2mell l : ll_def.ll pfrag_mell (map mell2ll l) -> mell l.
 Proof.
 intros pi.
 remember (map mell2ll l) as l0.
-revert l Heql0. induction pi; intros l' Heql0; subst;
-  try (destruct l'; inversion Heql0; destruct f; inversion H0; assumption).
+induction pi in l, Heql0 |- *; subst;
+  try (destruct l; destr_eq Heql0; destruct f; destr_eq Heql0; subst; now try (constructor; apply IHpi)).
 - symmetry in Heql0. decomp_map Heql0. subst.
-  destruct l1; inversion Heql4. destruct x; inversion Heql2. destruct x0; inversion Heql0. subst.
+  rewrite (map_eq_nil _ _ Heql4).
+  destruct x; destr_eq Heql2. destruct x0; destr_eq Heql0. subst.
   apply ax_r.
 - cbn in p.
   apply Permutation_Type_map_inv in p
@@ -150,40 +150,27 @@ revert l Heql0. induction pi; intros l' Heql0; subst;
   eapply ex_r; [ | eassumption ].
   apply IHpi. assumption.
 - symmetry in Heql0. decomp_map Heql0. subst. symmetry in Heql0.
-  destruct (mell2ll_map_wn_inv _ _ Heql0) as (l' & -> & ->).
-  apply Permutation_Type_map_inv in p as [l'' ->].
-  eapply (@ex_r (l0 ++ map wn l'' ++ l5)).
+  destruct (mell2ll_map_wn_inv _ _ Heql0) as [l [-> ->]].
+  apply Permutation_Type_map_inv in p as [l' ->].
+  eapply (@ex_r (l3 ++ map wn l' ++ l6)).
   + apply IHpi. list_simpl. rewrite mell2ll_map_wn. reflexivity.
   + symmetry. apply Permutation_app_head, Permutation_app_tail, Permutation_map, Permutation_Type_Permutation, p.
 - discriminate f.
 - symmetry in Heql0. decomp_map Heql0. subst.
-  destruct x; inversion Heql2. subst.
+  destruct x; destr_eq Heql2. subst.
   eapply ex_r; [ apply tens_r | ].
   + apply IHpi1. reflexivity.
   + apply IHpi2. reflexivity.
   + apply Permutation_cons, Permutation_app_comm. reflexivity.
-- destruct l'; inversion Heql0. destruct f; inversion H0. subst.
-  apply parr_r, IHpi. reflexivity.
-- destruct l'; inversion Heql0. destruct f; inversion H0. subst.
-  apply mell2ll_map_wn_inv in H1 as (l'' & -> & ->).
+- destruct l; destr_eq Heql0. destruct f; destr_eq Heql0. subst.
+  apply mell2ll_map_wn_inv in H as [l' [-> ->]].
   apply oc_r, IHpi. cbn. rewrite mell2ll_map_wn. reflexivity.
-- destruct l'; inversion Heql0. destruct f; inversion H0. subst.
-  apply de_r, IHpi. reflexivity.
-- destruct l'; inversion Heql0. destruct f; inversion H0. subst.
-  apply wk_r, IHpi. reflexivity.
-- symmetry in Heql0; decomp_map Heql0. subst.
-  destruct x; inversion Heql2. subst.
-  apply co_r, IHpi. reflexivity.
 - discriminate f.
 - destruct a.
 Qed.
 
 Lemma inhmellfrag2mell l : inhabited (ll_def.ll pfrag_mell (map mell2ll l)) -> mell l.
-Proof.
-assert (inhabited (ll_def.ll pfrag_mell (map mell2ll l)) -> inhabited (mell l)) as Hi
-  by apply inhabited_covariant, mellfrag2mell.
-intros [H]%Hi. exact H.
-Qed.
+Proof. intros [pi]%(inhabited_covariant (mellfrag2mell _)). exact pi. Qed.
 
 
 (** ** 6. import properties *)
@@ -200,10 +187,8 @@ Qed.
 
 Lemma cut_r A l1 l2 : mell (A :: l1) -> mell (dual A :: l2) -> mell (l1 ++ l2).
 Proof.
-intros [pi1]%mell2mellfrag [pi2]%mell2mellfrag.
-apply inhmellfrag2mell. constructor.
-rewrite map_app.
-eapply ll_cut.cut_r_axfree; [ intros [] | rewrite mell2ll_dual | ]; eassumption.
+intros [pi1]%mell2mellfrag [pi2]%mell2mellfrag. apply mellfrag2mell.
+rewrite map_app. eapply ll_cut.cut_r_axfree; [ intros [] | rewrite mell2ll_dual | ]; eassumption.
 Qed.
 
 End Atoms.
